Hoare/TerminationTriple.thy
@@ -567,57 +567,21 @@ using return_case2 apply force
 done
 done
 
-(*
 lemma using_gas_triple3 :
-   "triple {} (all_perhaps_less_gas g ** \<langle>g > 0\<rangle> ** continuing) {}
-    (all_with_less_gas g  ** \<langle>g-1 > 0\<rangle> ** continuing 
+   "triple {} (all_perhaps_less_gas g ** continuing
+    ## all_with_less_gas g ** not_continuing **
+      (delegating ## calling ## creating)
+    ## all_perhaps_less_gas g ** not_continuing **
+       (failing ## returning  ## destructing)) {}
+    (all_with_less_gas g ** continuing 
     ## all_with_less_gas g ** not_continuing **
       (delegating ## calling ## creating)
     ## all_perhaps_less_gas g ** not_continuing **
        (failing ## returning  ## destructing))"
-apply(auto simp add: triple_def)
- apply(rule_tac x = 1 in exI)
- apply(case_tac presult; auto)
-apply (simp add:sep_add_def  program_sem.simps next_state_def)
-apply (case_tac "vctx_next_instruction x1 co_ctx")
-apply (auto simp add:case_1 meter_gas_check)
-apply (simp add: instruction_result_as_set_def)
-using case_2 apply force
-defer
-defer
-apply (simp add: instruction_result_as_set_def)
-using case_2 apply force
-using meter_gas_check apply force
-using meter_gas_check apply force
-apply (simp add: instruction_result_as_set_def)
-using case_2 apply force
-subgoal for co_ctx rest v1 inst
-apply (case_tac "instruction_sem v1 co_ctx inst"; auto)
-apply (simp add: instruction_result_as_set_def)
-using no_annotation_inst apply simp
-apply (case_tac x31; auto simp:simple)
-using call_case2 apply force
-using delegatecall_case2 apply force
-using create_case2 apply force
-using fail_case2 apply force
-using suicide_case2 apply force
-using return_case2 apply force
+using triple_stable using_gas_triple2
+apply force
 done
-subgoal for co_ctx rest v1 inst
-apply (case_tac "instruction_sem v1 co_ctx inst"; auto)
-apply (simp add: instruction_result_as_set_def)
-using normal_case2 apply simp
-using no_annotation_inst apply simp
-apply (case_tac x31; auto simp:simple)
-using call_case2 apply force
-using delegatecall_case2 apply force
-using create_case2 apply force
-using fail_case2 apply force
-using suicide_case2 apply force
-using return_case2 apply force
-done
-done
-*)
+
 lemma test :
   " all_perhaps_less_gas (if 0 \<le> g then g else 0) **
        \<langle> 0 < (if 0 \<le> g then g else 0) \<rangle> =
@@ -630,6 +594,11 @@ lemma false_zero : "\<langle> False \<rangle> = zero"
 apply (auto simp:zero_def pure_def)
 done
 
+lemma simple_triple :
+  "(\<forall>x. p x \<longrightarrow> r x) \<Longrightarrow>
+   triple {} p {} r"
+  by (simp add: pre_imp triple_tauto)
+
 lemma termination_triple :
    "\<exists>y. y < 0 \<and>
     triple {} (all_perhaps_less_gas g ** continuing) {}
@@ -638,18 +607,160 @@ lemma termination_triple :
       (delegating ## calling ## creating)
     ## all_perhaps_less_gas g ** not_continuing **
        (failing ## returning  ## destructing)))"
-apply (rule loop_triple_int [of "\<lambda>g. all_perhaps_less_gas g ** continuing"
-  "all_with_less_gas g ** not_continuing **
+apply (rule loop_triple_int2 [of "\<lambda>g. all_perhaps_less_gas g ** continuing"
+  "\<lambda>g. all_with_less_gas g ** not_continuing **
       (delegating ## calling ## creating)
     ## all_perhaps_less_gas g ** not_continuing **
        (failing ## returning  ## destructing)" g])
+using using_gas_triple2 perhaps_less
+apply force
+apply auto
+apply (rule simple_triple)
+apply (auto simp:sep_add_def)
+  apply (smt all_with_less_gas_def sep_impL sep_three)
+  apply (smt all_with_less_gas_def sep_impL sep_three)
+  apply (smt all_with_less_gas_def sep_impL sep_three)
+  apply (smt all_perhaps_less_gas_def sep_impL sep_three)
+  apply (smt all_perhaps_less_gas_def sep_impL sep_three)
+  apply (smt all_perhaps_less_gas_def sep_impL sep_three)
+done
 
-using loop_triple_int [of "\<lambda>g. all_perhaps_less_gas g ** continuing"
-  "all_with_less_gas g ** not_continuing **
+lemma get_zero :
+   "(\<exists>y. y < 0 \<and> (\<forall>s. all_perhaps_less_gas y s)) \<Longrightarrow>
+    all_with_less_gas 0 s"
+apply (auto simp: all_perhaps_less_gas_def all_with_less_gas_def)
+  by fastforce
+
+lemma less_gas_memu :
+   "(rest ** all_with_less_gas g) (contexts_as_set v1 co_ctx) \<Longrightarrow>
+    vctx_memory_usage v1 \<ge> 0"
+  by (smt Un_upper2 all_with_less_gas_def get_condition1 sep_def)
+
+lemma less_gas_gas :
+   "(rest ** all_with_less_gas g) (contexts_as_set v1 co_ctx) \<Longrightarrow>
+    vctx_gas v1 < g"
+  by (smt Un_upper2 all_with_less_gas_def get_condition1 sep_def)
+
+lemma case_3 :
+assumes a :
+ "(rest ** all_with_less_gas g) (contexts_as_set x1 co_ctx)"
+shows  "(rest ** not_continuing ** all_with_less_gas g ** failing)
+           (insert (ContinuingElm False)
+             (insert
+               (ContractActionElm (ContractFail lst))
+               (contexts_as_set x1 co_ctx)))"
+proof -
+  let ?set =  "contexts_as_set x1 co_ctx"
+  let ?base =  "rest ** all_with_less_gas g"
+from a have "(?base ** not_continuing) (insert (ContinuingElm False) ?set)"
+  using context_cont1 not_cont_insert by presburger
+then have "(?base ** not_continuing)
+   (insert (ContinuingElm False) ?set-{ContractActionElm (ContractFail lst)})"
+  by (metis (full_types) Diff_empty Diff_insert2 context_cont context_cont1 contexts_as_set_def insert_minus state_element.distinct(685))
+then show ?thesis
+  by (metis failing_insert insert_commute sep_three set_pred.commute) 
+qed
+
+lemma no_gas :
+   "triple {} (all_with_less_gas 0 ** continuing) {}
+    (all_with_less_gas 0 ** not_continuing ** failing)"
+apply(auto simp add: triple_def)
+ apply(rule_tac x = 1 in exI)
+ apply(case_tac presult; auto)
+apply (simp add:sep_add_def  program_sem.simps next_state_def simple)
+apply (case_tac "vctx_next_instruction x1 co_ctx")
+apply (auto simp add:case_1 meter_gas_check simple)
+apply (simp add: instruction_result_as_set_def)
+using case_3 apply force
+using less_gas_memu less_gas_gas meter_gas_ge_0 apply smt
+using less_gas_memu less_gas_gas meter_gas_ge_0 apply smt
+using meter_gas_check apply force
+using less_gas_memu less_gas_gas meter_gas_ge_0
+apply (simp add: instruction_result_as_set_def)
+using case_3 apply force
+done
+
+lemma no_gas2 :
+   "y \<le> 0 \<Longrightarrow>
+    triple {} (all_with_less_gas y ** continuing) {}
+    (all_with_less_gas y ** not_continuing ** failing)"
+apply(auto simp add: triple_def)
+ apply(rule_tac x = 1 in exI)
+ apply(case_tac presult; auto)
+apply (simp add:sep_add_def  program_sem.simps next_state_def simple)
+apply (case_tac "vctx_next_instruction x1 co_ctx")
+apply (auto simp add:case_1 meter_gas_check simple)
+apply (simp add: instruction_result_as_set_def)
+using case_3 apply force
+using less_gas_memu less_gas_gas meter_gas_ge_0 apply smt
+using less_gas_memu less_gas_gas meter_gas_ge_0 apply smt
+using meter_gas_check apply force
+using less_gas_memu less_gas_gas meter_gas_ge_0
+apply (simp add: instruction_result_as_set_def)
+using case_3 apply force
+done
+
+lemma no_gas3 :
+   "y < 0 \<Longrightarrow>
+    triple {} (all_perhaps_less_gas y ** continuing) {}
+    (all_perhaps_less_gas y ** not_continuing ** failing)"
+using no_gas2 perhaps_less
+apply force
+done
+
+lemma triple_x :
+  "triple {} p {} (q1##r) \<Longrightarrow>
+   triple {} q1 {} q2 \<Longrightarrow>
+   triple {} p {} (q2##r)"
+proof -
+  assume a1: "triple {} p {} (q1 ## r)"
+  assume a2: "triple {} q1 {} q2"
+  have "triple {} zero {} (q2 ## r)"
+    by (metis zero_triple)
+  then have "triple {} q1 {} (q2 ## r)"
+    using a2 by (metis (no_types) sep_add_commute triple_three zero_add)
+  then have "\<exists>pa pb. triple {} pa {} (q2 ## r) \<and> triple {} pb {} (pa ## q2) \<and> triple {} p {} (pa ## pb)"
+    using a1 by (metis (no_types) sep_add_commute triple_stable zero_add zero_triple)
+  then show ?thesis
+  by (metis (full_types) sep_add_commute triple_three)
+qed
+
+
+lemma termination_triple2 :
+   "\<exists>y<0.
+    triple {} (all_perhaps_less_gas g ** continuing) {}
+    ((all_perhaps_less_gas y ** not_continuing ** failing) ##
+      (all_with_less_gas g ** not_continuing **
       (delegating ## calling ## creating)
     ## all_perhaps_less_gas g ** not_continuing **
-       (failing ## returning  ## destructing)" g]
-apply (auto simp:test false_zero zero_mul zero_add)
+       (failing ## returning  ## destructing)))"
+using termination_triple [of g]
+apply auto
+subgoal for y
+apply (rule exI [of _ y])
+apply auto
+using no_gas3 [of y]
+  triple_x [of "continuing ** all_perhaps_less_gas g"
+   "continuing ** all_perhaps_less_gas y"
+   "delegating ** not_continuing ** all_with_less_gas g ##
+      calling ** not_continuing ** all_with_less_gas g ##
+      creating ** not_continuing ** all_with_less_gas g ##
+      failing ** not_continuing ** all_perhaps_less_gas g ##
+      destructing ** not_continuing ** all_perhaps_less_gas g ##
+      returning ** not_continuing ** all_perhaps_less_gas g"
+   "all_perhaps_less_gas y ** not_continuing ** failing"]
+apply force
+done
+done
 
+lemma termination_triple3 :
+   "g \<ge> 0 \<Longrightarrow>
+    triple {} (all_perhaps_less_gas g ** continuing) {}
+    ( (all_with_less_gas g ** not_continuing **
+      (delegating ## calling ## creating)
+    ## all_perhaps_less_gas g ** not_continuing **
+       (failing ## returning  ## destructing)))"
+using termination_triple2 [of g]
+apply auto
 
 end
